frontend done

bin/web/compat.ml
@@ -1,0 +1,68 @@
+open Query.ExtractQuery
+
+let string_of_player = function
+  | White -> "white"
+  | Black -> "black"
+
+let string_of_piece = function
+  | King -> "king"
+  | Queen -> "queen"
+  | Rook -> "rook"
+  | Bishop -> "bishop"
+  | Knight -> "knight"
+
+let file_of_char = function
+  | 'a' -> file_a
+  | 'b' -> file_b
+  | 'c' -> file_c
+  | 'd' -> file_d
+  | 'e' -> file_e
+  | 'f' -> file_f
+  | 'g' -> file_g
+  | 'h' -> file_h
+  | _ -> invalid_arg "file_of_char"
+
+let string_of_file f =
+  match f with
+  | f when f = file_a -> "a"
+  | f when f = file_b -> "b"
+  | f when f = file_c -> "c"
+  | f when f = file_d -> "d"
+  | f when f = file_e -> "e"
+  | f when f = file_f -> "f"
+  | f when f = file_g -> "g"
+  | f when f = file_h -> "h"
+  | _ -> invalid_arg "char_of_file"
+
+let string_of_rank r =
+  match r with
+  | r when r = rank_1 -> "1"
+  | r when r = rank_2 -> "2"
+  | r when r = rank_3 -> "3"
+  | r when r = rank_4 -> "4"
+  | r when r = rank_5 -> "5"
+  | r when r = rank_6 -> "6"
+  | r when r = rank_7 -> "7"
+  | r when r = rank_8 -> "8"
+  | _ -> invalid_arg "char_of_rank"
+
+let rank_of_char = function
+  | '1' -> rank_1
+  | '2' -> rank_2
+  | '3' -> rank_3
+  | '4' -> rank_4
+  | '5' -> rank_5
+  | '6' -> rank_6
+  | '7' -> rank_7
+  | '8' -> rank_8
+  | _ -> invalid_arg "rank_of_char"
+
+let string_of_pos (f,r) =
+  string_of_file f ^ string_of_rank r
+
+let pos_of_string s =
+  if String.length s <> 2 then
+    invalid_arg "square_of_string";
+  let file = file_of_char s.[0] in
+  let rank = rank_of_char s.[1] in
+  (file, rank)
