bin/web/model.ml
@@ -1,0 +1,138 @@
+open Query.ExtractQuery
+
+module Model = struct
+
+  type editState = {
+    es_board : editBoard;
+    es_invalid : bool
+  }
+
+  type t =
+    | Edit of editState
+    | Query of chessState
+    | SelectingPlayer of chessState
+    | Play of chessState * strategy
+
+  let init_editState = {
+    es_board = init_edit;
+    es_invalid = false;
+  }
+
+  let init : t =
+    Edit init_editState
+
+end
+
+(* Action *)
+
+let user_step st str (mv : chessMove) =
+  match Lazy.force str with
+  | Abelard_strategy (_, strs) ->
+      (exec_ChessMove st (Obj.magic mv), strs (Obj.magic mv))
+  | Atom_strategy _ ->
+      failwith "Atom_strategy called unexpectedly"
+  | Eloise_strategy (_,_,_) ->
+      failwith "Eloise_strategy called unexpectedly"
+
+module Action = struct
+
+  type t =
+  | DragPiece of editMove
+  | TogglePlayer
+  | EditMode
+  | QueryMode
+  | PlayMode
+  | SelectPlayer of player
+  | SelectMove of chessMove
+  | AddPiece of piece * player * pos
+  | BlankBoard
+
+  let apply tb (a : t) (s : Model.t) : Model.t =
+    match s with
+    | Edit e ->
+      begin match a with
+      | DragPiece em -> Edit { e with es_board = execEditMove em e.es_board }
+      | TogglePlayer -> Edit { e with es_board = toggle_player e.es_board }
+      | EditMode -> Edit e
+      | QueryMode ->
+        begin match mk_KRvK_bound e.es_board with
+        | Success st -> Query st
+        | Error _msg -> Edit { e with es_invalid = true }
+        end
+      | PlayMode ->
+        begin match mk_KRvK_bound e.es_board with
+        | Success st -> SelectingPlayer st
+        | Error _msg -> Edit { e with es_invalid = true }
+        end
+      | SelectPlayer _ -> Edit e
+      | SelectMove _ -> Edit e
+      | AddPiece(pc, pl, pos) ->
+          Model.Edit { e with es_board =
+            { e.es_board with edit_board = place_piece pl pc pos e.es_board.edit_board }
+          }
+      | BlankBoard -> Edit {
+          es_board = { e.es_board with edit_board = blank_board };
+          es_invalid = false }
+      end
+    | Query st ->
+      begin match a with
+      | DragPiece em ->
+        begin match lookup_piece em.orig st.board0 with
+        | Some (_,pc) ->
+          let m = { piece0 = pc; origin = em.orig; dest = em.dest0 } in
+          Query (exec_ChessMove st m)
+        | None -> s
+        end
+      | TogglePlayer -> s
+      | EditMode -> Edit {
+          es_board =
+            editBoard_of_PreChessState (preChessState_of_ChessState st);
+          es_invalid = false;
+        }
+      | QueryMode -> Query st
+      | PlayMode -> SelectingPlayer st
+      | SelectPlayer _ -> Query st
+      | SelectMove m -> Query (exec_ChessMove st m)
+      | AddPiece(_,_,_) -> s
+      | BlankBoard -> s
+      end
+    | SelectingPlayer st ->
+      begin match a with
+      | DragPiece _ -> SelectingPlayer st
+      | TogglePlayer -> SelectingPlayer st
+      | EditMode -> Edit {
+          es_board =
+            editBoard_of_PreChessState (preChessState_of_ChessState st);
+          es_invalid = false;
+        }
+      | QueryMode -> Query st
+      | PlayMode -> SelectingPlayer st
+      | SelectPlayer pl -> Play (st, tb_strat (opp0 pl) st tb)
+      | SelectMove _ -> SelectingPlayer st
+      | AddPiece(_,_,_) -> SelectingPlayer st
+      | BlankBoard -> SelectingPlayer st
+      end
+    | Play (st, str) ->
+      begin match a with
+      | DragPiece em ->
+        begin match lookup_piece em.orig st.board0 with
+        | Some (_,pc) ->
+          let m = { piece0 = pc; origin = em.orig; dest = em.dest0 } in
+          let (st', str') = user_step st str m in
+          Play (st', str')
+        | None -> s
+        end
+      | TogglePlayer -> Play (st, str)
+      | EditMode -> Edit {
+          es_board =
+            editBoard_of_PreChessState (preChessState_of_ChessState st);
+          es_invalid = false;
+        }
+      | QueryMode -> Query st
+      | PlayMode -> Play (st, str)
+      | SelectPlayer _ -> Play (st, str)
+      | SelectMove _ -> Play (st, str)
+      | AddPiece(_,_,_) -> Play (st, str)
+      | BlankBoard -> Play (st, str)
+      end
+end
