bin/web/util.ml
@@ -1,0 +1,12 @@
+open Js_of_ocaml
+open Compat
+
+let create_element tag =
+  Dom_html.document##createElement (Js.string tag)
+let append_child parent child =
+  Dom.appendChild parent child
+let set_style el key value = ignore
+  (el##.style##setProperty (Js.string key) (Js.string value) Js.undefined)
+let log x = Firebug.console##log x
+let log_player pl =
+  log (string_of_player pl)
