bin/query/ExtractQuery.v
@@ -7,18 +7,141 @@ Require Import Games.Util.Dec.
 Require Import Chess.Util.Fin.
 Extraction Language OCaml.
 
+Require Import Games.Game.Game.
+Require Import Games.Game.Strategy.
+Require Import Games.Game.Player.
 Require Import Chess.TB.MakeState.
 Require Import Chess.Chess.Chess.
 Require Import TBGen.StratSymTB.TB.
 Require Import TBGen.StratSymTB.OCamlTB.
 
+Require Import List.
+Import ListNotations.
+
 Set Warnings "-extraction-default-directory".
 
 Definition query : OCamlTablebase ChessGame ->
-  ChessState -> option (Player.Player * nat) :=
+  ChessState -> option (Player * nat) :=
   query_TB.
 
+Fixpoint max_by {X} (x_leb : X -> X -> bool) (xs : list X) : option X :=
+  match xs with
+  | [] => None
+  | x :: xs' =>
+    match max_by x_leb xs' with
+    | None => Some x
+    | Some y => if x_leb x y then Some y else Some x
+    end
+  end.
+
+Lemma max_by_ne_Some {X} x_leb (xs : list X) (pf : xs <> []) :
+  { x : X & max_by x_leb xs = Some x }.
+Proof.
+  destruct xs.
+  - elim (pf eq_refl).
+  - simpl.
+    destruct (max_by x_leb xs).
+    + destruct (x_leb x x0).
+      * exists x0; reflexivity.
+      * exists x; reflexivity.
+    + exists x; reflexivity.
+Defined.
+
+Definition max_by_ne {X} x_leb (xs : list X) (pf : xs <> []) : X :=
+  projT1 (max_by_ne_Some x_leb xs pf).
+
+Lemma move_enum_all_ne {G} {s : Game.GameState G} (s_res : atomic_res s = None) : enum_moves s <> [].
+Proof.
+  intro pf.
+  destruct (nil_atomic_res pf); congruence.
+Qed.
+
+Definition p_leb (pl : Player) (r1 r2 : option (Player * nat)) : bool :=
+  match pl with
+  | White =>
+    match r1, r2 with
+    | Some (Black, m), Some (Black, n) => Nat.leb m n
+    | Some (Black, _), _ => true
+    | None, None => true
+    | None, Some (White, _) => true
+    | Some (White, m), Some (White, n) => Nat.leb n m
+    | _, _ => false
+    end
+  | Black =>
+    match r1, r2 with
+    | Some (White, m), Some (White, n) => Nat.leb m n
+    | Some (White, _), _ => true
+    | None, None => true
+    | None, Some (Black, _) => true
+    | Some (Black, m), Some (Black, n) => Nat.leb n m
+    | _, _ => false
+    end
+  end.
+
+Definition atomic_chess_res_fast
+  (s : ChessState) : option Result :=
+  let pl := chess_to_play s in
+  match enum_chess_moves s with
+  | [] =>
+    match is_threatened_byb (board s) (king s pl) (opp pl) with
+    | true => Some (Win (opp pl))
+    | false => Some Draw
+    end
+  | _ :: _ => None
+  end.
+
+Lemma atomic_chess_res_fast_correct s :
+  atomic_chess_res_fast s =
+  @atomic_res ChessGame s.
+Proof.
+  simpl.
+  unfold atomic_chess_res_fast, atomic_chess_res.
+  destruct enum_chess_moves; auto.
+  destruct dec as [chk|no_chk]; unfold in_check in *.
+  - specialize (chk (king s (chess_to_play s))
+      (lookup_king s _)).
+    rewrite is_threatened_byb_iff in chk.
+    rewrite chk; auto.
+  - destruct is_threatened_byb eqn:Hthr; auto.
+    rewrite <- is_threatened_byb_iff in Hthr.
+    elim no_chk; intros pos Hpos.
+    apply s in Hpos; subst; auto.
+Qed.
+
+CoFixpoint tb_strat pl (s : ChessState)
+  (tb : OCamlTablebase ChessGame) :
+  @strategy ChessGame pl s.
+Proof.
+  - destruct (atomic_chess_res_fast s) eqn:s_res;
+    rewrite atomic_chess_res_fast_correct in s_res.
+    + eapply atom_strategy; eauto.
+    + destruct (player_id_or_opp_r_t (@to_play ChessGame s) pl) as [s_play|s_play].
+      * pose (m := max_by_ne
+          (fun m1 m2 => p_leb pl
+             (query_TB tb (@exec_move ChessGame s m1))
+             (query_TB tb (@exec_move ChessGame s m2))
+          ) (@enum_moves ChessGame s) (move_enum_all_ne s_res)).
+        exact (eloise_strategy s_res s_play m (@tb_strat pl _ tb)).
+      * exact (abelard_strategy s_res s_play (fun m =>
+          @tb_strat pl _ tb)).
+Defined.
+
+Definition dump_board (b : Board) : list (Pos * Piece * Player) :=
+  let m := MaterialPositions.mp_of_board b in
+  flat_map (fun pc => map (fun pos => (pos, pc, White))
+    (m White pc)) all_piece ++
+  flat_map (fun pc => map (fun pos => (pos, pc, Black))
+    (m Black pc)) all_piece.
+
 Extraction "ExtractQuery.ml"
+  p_leb
+  tb_strat
+  dump_board
+  enum_chess_moves
+  buildMove
+  execEditMove
+  toggle_player
+  init_edit
   mk_KRvK_bound
   exec_ChessMove
   query
